subsume LabeledDynamicNet.v into DynamicNet.v

core/DynamicNet.v
@@ -1,7 +1,7 @@
 Require Import List.
 Require Import Arith.
+Require Import InfSeqExt.infseq.
 Import ListNotations.
-
 
 Section Dynamic.
   Variable addr : Type. (* must be finite, decidable *)
@@ -11,6 +11,8 @@ Section Dynamic.
   Variable data : Type.
   Variable timeout : Type.
   Variable timeout_eq_dec : forall x y : timeout, {x = y} + {x <> y}.
+  Variable label : Type.
+  Variable label_eq_dec : forall x y : label, {x = y} + {x <> y}.
 
   Variable start_handler : addr -> list addr -> data * list (addr * payload) * list timeout.
 
@@ -18,6 +20,15 @@ Section Dynamic.
 
   Variable recv_handler : addr -> addr -> data -> payload -> res.
   Variable timeout_handler : addr -> data -> timeout -> res.
+  Variable recv_handler_l : addr -> addr -> data -> payload -> (res * label).
+  Variable timeout_handler_l : addr -> data -> timeout -> (res * label).
+
+  Variable recv_handler_labeling :
+    forall src dst st p,
+      recv_handler src dst st p = fst (recv_handler_l src dst st p).
+  Variable timeout_handler_labeling :
+    forall h st t,
+      timeout_handler h st t = fst (timeout_handler_l h st t).
 
   (* can clients send this payload? disallows forgery *)
   Variable client_payload : payload -> Prop.
@@ -40,7 +51,7 @@ Section Dynamic.
   | e_recv : msg -> event
   | e_timeout : addr -> timeout -> event
   | e_fail : addr -> event.
- 
+
   Record global_state :=
     { nodes : list addr;
       failed_nodes : list addr;
@@ -187,4 +198,81 @@ Section Dynamic.
                |} ->
         extra_constraints gst' ->
         step_dynamic gst gst'.
+
+  Inductive labeled_step_dynamic : global_state -> label -> global_state -> Prop :=
+  | LTimeout :
+      forall gst gst' h st t lb st' ms newts clearedts,
+        In h (nodes gst) ->
+        ~ In h (failed_nodes gst) ->
+        sigma gst h = Some st ->
+        In t (timeouts gst h) ->
+        timeout_handler_l h st t = (st', ms, newts, clearedts, lb) ->
+        gst' = (apply_handler_result
+                  h
+                  (st', ms, newts, t :: clearedts)
+                  (e_timeout h t)
+                  gst) ->
+        extra_constraints gst' ->
+        labeled_step_dynamic gst lb gst'
+  | LDeliver_node :
+      forall gst gst' m h d xs ys ms lb st newts clearedts,
+        msgs gst = xs ++ m :: ys ->
+        h = fst (snd m) ->
+        In h (nodes gst) ->
+        ~ In h (failed_nodes gst) ->
+        sigma gst h = Some d ->
+        recv_handler_l (fst m) h d (snd (snd m)) = (st, ms, newts, clearedts, lb) ->
+        gst' = apply_handler_result
+                 h
+                 (st, ms, newts, clearedts)
+                 (e_recv m)
+                 (update_msgs gst (xs ++ ys)) ->
+        extra_constraints gst' ->
+        labeled_step_dynamic gst lb gst'.
+
+  Record occurrence := { occ_gst : global_state ; occ_label : label }.
+
+  Definition enabled (l : label) (gst : global_state) : Prop :=
+    exists gst', labeled_step_dynamic gst l gst'.
+
+  Definition l_enabled (l : label) (occ : occurrence) : Prop :=
+    enabled l (occ_gst occ).
+
+  Definition occurred (l : label) (occ :occurrence) : Prop := l = occ_label occ.
+
+  Definition inf_enabled (l : label) (s : infseq occurrence) : Prop :=
+    inf_often (now (l_enabled l)) s.
+
+  Definition inf_occurred (l : label) (s : infseq occurrence) : Prop :=
+    inf_often (now (occurred l)) s.
+
+  Definition strong_local_fairness (s : infseq occurrence) : Prop :=
+    forall l : label, inf_enabled l s -> inf_occurred l s.
+
+  Lemma strong_local_fairness_invar :
+    forall e s, strong_local_fairness (Cons e s) -> strong_local_fairness s.
+  Proof.
+    unfold strong_local_fairness. unfold inf_enabled, inf_occurred, inf_often.
+    intros e s fair a alev.
+    assert (alevt_es: always (eventually (now (l_enabled a))) (Cons e s)).
+    constructor.
+    constructor 2. destruct alev; assumption.
+    simpl. assumption.
+    clear alev. generalize (fair a alevt_es); clear fair alevt_es.
+    intro fair; case (always_Cons fair); trivial.
+  Qed.
+
+  CoInductive lb_execution : infseq occurrence -> Prop :=
+    Cons_lb_exec : forall (o o' : occurrence) (s : infseq occurrence),
+      labeled_step_dynamic (occ_gst o) (occ_label o) (occ_gst o') ->
+      lb_execution (Cons o' s) ->
+      lb_execution (Cons o (Cons o' s)).
+
+  Lemma lb_execution_invar :
+    forall x s, lb_execution (Cons x s) -> lb_execution s.
+  Proof.
+    intros x s e. change (lb_execution (tl (Cons x s))).
+    destruct e; simpl. assumption.
+  Qed.
+
 End Dynamic.
